Remove debug printing

extraction/tests/RecordExtractionLiquidityTests.v
@@ -33,15 +33,17 @@ Module RecordsWithoutPrimitiveProjections.
   
   Definition proj_A_printed := 
     Eval vm_compute in unwrap_sum (liquidity_extract_single TT_defs [] true "" "" proj_A_quoted).
-  Example A_printed_as_type_alias : proj_A_printed =?
-<$ "";
-"";
-"type a = nat";
-"";
-"let proj_A (a : a) = a";
-"";
-"" $>.
-  Proof. unfold proj_A_printed. reflexivity. Qed.
+
+  Example A_printed_as_type_alias :
+    proj_A_printed =?
+    <$ "";
+    "";
+    "type a = nat";
+    "";
+    "let proj_A (a : a) = a";
+    "";
+    "" $>.
+  Proof. reflexivity. Qed.
   
   Definition constructA : A := 
     let a1 := {| x:= 0 |} in
@@ -52,18 +54,20 @@ Module RecordsWithoutPrimitiveProjections.
 
   Definition constructA_printed := 
     Eval vm_compute in unwrap_sum (liquidity_extract_single TT_defs [] true "" "" constructA_quoted).
-  Print constructA_printed.
-  Example constructA_omits_constructor : constructA_printed =?
-<$
-"";
-"";
-"type a = nat";
-"";
-"let constructA  = let a1 = O in ";
-"let a2 = O in ";
-"a1";
-"";
-"" $>. Proof. unfold constructA_printed. reflexivity. Qed.
+
+  Example constructA_omits_constructor :
+    constructA_printed =?
+    <$
+    "";
+    "";
+    "type a = nat";
+    "";
+    "let constructA  = let a1 = O in ";
+    "let a2 = O in ";
+    "a1";
+    "";
+    "" $>.
+  Proof. reflexivity. Qed.
 
   Record B := build_B {
     y : nat;
@@ -77,19 +81,20 @@ Module RecordsWithoutPrimitiveProjections.
 
   Definition proj_B_printed :=
     Eval vm_compute in unwrap_sum (liquidity_extract_single TT_defs [] true "" "" proj_B_quoted).
-    Print proj_B_printed.
-    Example B_printed_as_type_alias : proj_B_printed =?
-<$"";
-"";
-"type b = {";
-"y : nat;";
-"z : nat";
-"}";
-"";
-"let proj_B (b : b) = b.z";
-"";
-"" $>.
-  Proof. unfold proj_B_printed. reflexivity. Qed.
+
+  Example B_printed_as_type_alias :
+    proj_B_printed =?
+    <$"";
+    "";
+    "type b = {";
+    "y : nat;";
+    "z : nat";
+    "}";
+    "";
+    "let proj_B (b : b) = b.z";
+    "";
+    "" $>.
+  Proof. reflexivity. Qed.
     
   Definition constructB : B := 
     let B1 := {| y:= 0; z:=0 |} in
@@ -100,20 +105,22 @@ Module RecordsWithoutPrimitiveProjections.
 
   Definition constructB_printed := 
     Eval vm_compute in unwrap_sum (liquidity_extract_single TT_defs [] true "" "" constructB_quoted).
-  Print constructB_printed.
-  Example constructB_uses_record_syntax : constructB_printed =?
-<$"";
-"";
-"type b = {";
-"y : nat;";
-"z : nat";
-"}";
-"";
-"let constructB  = let b1 = {y = O; z = O} in ";
-"let b2 = {y = O; z = O} in ";
-"b1";
-"";
-"" $>. Proof. unfold constructB_printed. reflexivity. Qed.
+
+  Example constructB_uses_record_syntax :
+    constructB_printed =?
+    <$"";
+    "";
+    "type b = {";
+    "y : nat;";
+    "z : nat";
+    "}";
+    "";
+    "let constructB  = let b1 = {y = O; z = O} in ";
+    "let b2 = {y = O; z = O} in ";
+    "b1";
+    "";
+    "" $>.
+  Proof. reflexivity. Qed.
 
 End RecordsWithoutPrimitiveProjections.
 
@@ -132,15 +139,16 @@ Module RecordWithPrimitiveProjections.
   Definition proj_A_printed := 
     Eval vm_compute in unwrap_sum (liquidity_extract_single TT_defs [] true "" "" proj_A_quoted).
 
-  Example A_printed_as_type_alias : proj_A_printed =?
-<$"";
-"";
-"type a = nat";
-"";
-"let proj_A (a : a) = a";
-"";
-"" $>.
-  Proof. unfold proj_A_printed. reflexivity. Qed.
+  Example A_printed_as_type_alias :
+    proj_A_printed =?
+    <$"";
+    "";
+    "type a = nat";
+    "";
+    "let proj_A (a : a) = a";
+    "";
+    "" $>.
+  Proof. reflexivity. Qed.
 
   Definition constructA : A := 
     let a1 := {| x:= 0 |} in
@@ -151,17 +159,19 @@ Module RecordWithPrimitiveProjections.
 
   Definition constructA_printed := 
     Eval vm_compute in unwrap_sum (liquidity_extract_single TT_defs [] true "" "" constructA_quoted).
-  Print constructA_printed.
-  Example constructA_omits_constructor : constructA_printed =?
-<$"";
-"";
-"type a = nat";
-"";
-"let constructA  = let a1 = O in ";
-"let a2 = O in ";
-"a1";
-"";
-"" $>. Proof. reflexivity. Qed.
+
+  Example constructA_omits_constructor :
+    constructA_printed =?
+    <$"";
+    "";
+    "type a = nat";
+    "";
+    "let constructA  = let a1 = O in ";
+    "let a2 = O in ";
+    "a1";
+    "";
+    "" $>.
+  Proof. reflexivity. Qed.
 
   Record B := build_B {
     y : nat;
@@ -171,25 +181,23 @@ Module RecordWithPrimitiveProjections.
   Definition proj_B (b : B) := b.(z).
 
   MetaCoq Quote Recursively Definition proj_B_quoted := proj_B.
-  (* Print proj_B_quoted. *)
 
   Definition proj_B_printed :=
     Eval vm_compute in unwrap_sum (liquidity_extract_single TT_defs [] true "" "" proj_B_quoted).
 
-    Print proj_B_printed.
-
-    Example B_printed_as_type_alias : proj_B_printed =?
-<$"";
-"";
-"type b = {";
-"y : nat;";
-"z : nat";
-"}";
-"";
-"let proj_B (b : b) = b.z";
-"";
-"" $>.
-  Proof. unfold proj_B_printed. reflexivity. Qed.
+  Example B_printed_as_type_alias :
+    proj_B_printed =?
+    <$"";
+    "";
+    "type b = {";
+    "y : nat;";
+    "z : nat";
+    "}";
+    "";
+    "let proj_B (b : b) = b.z";
+    "";
+    "" $>.
+  Proof. reflexivity. Qed.
   
 
   Definition constructB : B := 
@@ -201,19 +209,21 @@ Module RecordWithPrimitiveProjections.
 
   Definition constructB_printed := 
     Eval vm_compute in unwrap_sum (liquidity_extract_single TT_defs [] true "" "" constructB_quoted).
-  Print constructB_printed.
-  Example constructB_uses_record_syntax : constructB_printed =?
-<$ "";
-"";
-"type b = {";
-"y : nat;";
-"z : nat";
-"}";
-"";
-"let constructB  = let b1 = {y = O; z = O} in ";
-"let b2 = {y = O; z = O} in ";
-"b1";
-"";
-"" $>. Proof. unfold constructB_printed. reflexivity. Qed.
+
+  Example constructB_uses_record_syntax :
+    constructB_printed =?
+    <$ "";
+    "";
+    "type b = {";
+    "y : nat;";
+    "z : nat";
+    "}";
+    "";
+    "let constructB  = let b1 = {y = O; z = O} in ";
+    "let b2 = {y = O; z = O} in ";
+    "b1";
+    "";
+    "" $>.
+  Proof. reflexivity. Qed.
 
 End RecordWithPrimitiveProjections.
