embedding/theories/CertifyingTranslate.v
@@ -41,7 +41,7 @@ Definition my_negb_syn :=
           | True -> False
           | False -> True |].
 
-Compute expr_to_tc Σ (indexify nil my_negb_syn).
+(* Compute expr_to_tc Σ (indexify nil my_negb_syn). *)
 
 (** We translate and unquote using the ConCert embedding feature *)
 MetaCoq Unquote Definition my_negb := (expr_to_tc Σ (indexify nil my_negb_syn)).
